src/tls/Handshake.fst
@@ -574,7 +574,7 @@ let server_ClientHello hs offer =
         if mode.Nego.n_protocol_version = TLS_1p3
         then 
           begin
-          trace "Derive handshake keys";
+          trace "derive handshake keys";
           let hs_keys = KeySchedule.ks_server_13_sh hs.ks digestServerHello (* digestServerHello *)  in
           register hs hs_keys;
           // We will start using the HTKs later (after sending SH, and after receiving 0RTT traffic)
